begin scripting the Compiler.v file

tools/compiler_expand.ml
@@ -1,0 +1,62 @@
+type is_partial = TOTAL | PARTIAL;;
+type when_triggered = Always | Option of string;;
+
+let passes =
+[|
+TOTAL, (Option "optim_tailcalls"), (Some "Tail calls"), "Tailcall";
+PARTIAL, Always, (Some "Inlining"), "Inlining";
+TOTAL, (Option "profile_arcs"), (Some "Profiling insertion"), "Profiling";
+TOTAL, (Option "branch_probabilities"), (Some "Profiling use"), "ProfilingExploit";
+TOTAL, (Option "optim_move_loop_invariants"), (Some "Inserting initial nop"), "FirstNop";
+TOTAL, Always, (Some "Renumbering"), "Renumber";
+PARTIAL, (Option "optim_duplicate"),  (Some "Tail-duplicating"), "Duplicate";
+TOTAL, Always, (Some "Renumbering pre constprop"), "Renumber";
+TOTAL, (Option "optim_constprop"), (Some "Constant propagation"), "Constprop";
+PARTIAL, (Option "optim_move_loop_invariants"), (Some "LICM"), "LICM";
+TOTAL, (Option "optim_move_loop_invariants"), (Some "Renumbering pre CSE"), "Renumber";
+PARTIAL, (Option "optim_CSE"), (Some "CSE"), "CSE";
+TOTAL, (Option "optim_CSE2"), (Some "CSE2"), "CSE2";
+PARTIAL, (Option "optim_CSE3"), (Some "CSE3"), "CSE3";
+TOTAL, (Option "optim_forward_moves"), (Some "Forwarding moves"), "ForwardMoves";
+PARTIAL, (Option "optim_redundancy"), (Some "Redundancy elimination"), "Deadcode";
+TOTAL, (Option "all_loads_nontrap"), None, "Allnontrap";
+PARTIAL, Always, (Some "Unused globals"), "Unusedglob"
+|];;
+
+let totality = function TOTAL -> "total" | PARTIAL -> "partial";;
+
+let print_transf oc =
+  Array.iteri
+    (fun i (partial, trigger, time_label, pass_name) ->
+      output_string oc (match partial with
+                        | TOTAL -> "   @@ "
+                        | PARTIAL -> "  @@@ ");
+      (match trigger with
+       | Always -> ()
+       | Option s ->
+          Printf.fprintf oc "%s_if Compopts.%s " (totality partial) s);
+      output_char oc '(';
+      (match time_label with
+       | None -> ()
+       | Some s ->
+          Printf.fprintf oc "time \"%s\" " s);
+      Printf.fprintf oc "%s.transf_program)\n" pass_name;
+      Printf.fprintf oc "   @@ print (print_RTL %d)\n" (succ i)
+    ) passes;;
+    
+if (Array.length Sys.argv)<>3
+then exit 1;;
+
+let filename_in = Sys.argv.(1) and filename_out = Sys.argv.(2) in
+    let ic = open_in filename_in and oc = open_out filename_out in
+    try
+      while true
+      do
+        let line = input_line ic in
+        if line = "EXPAND_TRANSF_PROGRAM"
+        then print_transf oc
+        else (output_string oc line;
+              output_char oc '\n')
+      done
+    with End_of_file ->
+      (close_in ic; close_out oc);;
